transformations/Class2Relational_TUPLE_SP/theorems/Elements.v
@@ -97,9 +97,11 @@ Proof.
 
     {
       unfold instantiateRuleOnPiece.
+      unfold traceRuleOnPiece.
+      rewrite map_flat_map.
       simpl.
       unfold EvalUserExpressions.evalIterator.
-      rewrite HeqR at 2 ; simpl.
+      rewrite HeqR at 1 ; simpl.
       rewrite List.app_nil_r.
       unfold instantiateIterationOnPiece ; simpl.
       rewrite HeqR ; unfold Syntax.r_outputPattern ; simpl.
